Allow more swaps than were allowed before :) See msg.
Some lemmas broke due to this change and will be updated in upcoming
commits.

We now allow entire blocks of code to move past each other, as long as
they satisfy the r/w requirements. We explicitly DO NOT perform
block/unblock, and leave that to the user of this transformation to
do. However, if it is possible to move two [code]s objects past each
other, this will allow it.

At the moment, this is fairly limited, since we don't have very
precise definition for taking multiple [rw_set]s in series, but once
we have them, this should allow us to move larger chunks of code
across.

vale/code/lib/transformers/Vale.Transformers.InstructionReorder.fst
@@ -1024,9 +1024,11 @@ let wrap_ss (f:machine_state -> machine_state) : st unit =
   set (f s)
 
 let wrap_sos (f:machine_state -> option machine_state) : st unit =
-  let open Vale.X64.Machine_Semantics_s in
-  s <-- get;
-  apply_option (f s) set
+  fun s -> (
+      match f s with
+      | None -> (), { s with ms_ok = false }
+      | Some s' -> (), s'
+    )
 
 let lemma_feq_bounded_effects (rw:rw_set) (f1 f2:st unit) :
   Lemma
@@ -1159,35 +1161,10 @@ and rw_set_of_codes (c:safely_bounded_codes) : rw_set =
       (rw_set_of_code x)
       (rw_set_of_codes xs)
 
-/// Given that we can perform simple swaps between instructions, we
-/// can do swaps between [code]s.
-
-let code_exchange_allowed (c1 c2:code) : pbool =
-  match c1, c2 with
-  | Ins i1, Ins i2 -> ins_exchange_allowed i1 i2
-  | _ -> ffalse "non instruction swaps conservatively disallowed"
-
-#push-options "--initial_fuel 3 --max_fuel 3 --max_ifuel 0"
-let lemma_code_exchange (c1 c2 : code) (fuel:nat) (s1 s2 : machine_state) :
+let lemma_bounded_code (c:safely_bounded_code) (fuel:nat) :
   Lemma
-    (requires (
-        !!(code_exchange_allowed c1 c2) /\
-        (equiv_states s1 s2) /\
-        (Some? (machine_eval_codes [c1; c2] fuel s1))))
-    (ensures (
-        (Some? (machine_eval_codes [c2; c1] fuel s2)) /\
-        (let Some s1', Some s2' =
-           machine_eval_codes [c1; c2] fuel s1,
-           machine_eval_codes [c2; c1] fuel s2 in
-         equiv_states_or_both_not_ok s1' s2'))) =
-  let Some s1', Some s2' =
-    machine_eval_codes [c1; c2] fuel s1,
-    machine_eval_codes [c2; c1] fuel s2 in
-  match c1, c2 with
-  | Ins i1, Ins i2 ->
-    lemma_instruction_exchange i1 i2 s1 s2
-  | _ -> ()
-#pop-options
+    (ensures (bounded_effects (rw_set_of_code c) (wrap_sos (machine_eval_code c fuel)))) =
+  admit ()
 
 /// Not-ok states lead to erroring states upon execution
 
@@ -1233,6 +1210,60 @@ and lemma_not_ok_propagate_while (c:code{While? c}) (fuel:nat) (s:machine_state)
       lemma_not_ok_propagate_code body (fuel - 1) s
     )
   )
+
+/// Given that we can perform simple swaps between instructions, we
+/// can do swaps between [code]s.
+
+let code_exchange_allowed (c1 c2:safely_bounded_code) : pbool =
+  rw_exchange_allowed (rw_set_of_code c1) (rw_set_of_code c2)
+  /+> normal (" for instructions " ^ fst (print_code c1 0 gcc) ^ " and " ^ fst (print_code c2 0 gcc))
+
+let lemma_run_2_to_run2 (f1 f2:st unit) (s:machine_state) :
+  Lemma
+    (requires (
+        (s.ms_ok) /\
+        (run f1 s).ms_ok /\
+        (run f2 (run f1 s)).ms_ok
+    ))
+    (ensures (run2 f1 f2 s == run f2 (run f1 s))) = ()
+
+#push-options "--z3rlimit 20"
+let lemma_code_exchange_allowed (c1 c2 : safely_bounded_code) (fuel:nat) (s : machine_state) :
+  Lemma
+    (requires (
+        !!(code_exchange_allowed c1 c2) /\
+        not (erroring_option_state (machine_eval_codes [c1; c2] fuel s))))
+    (ensures (
+        equiv_option_states
+          (machine_eval_codes [c1; c2] fuel s)
+          (machine_eval_codes [c2; c1] fuel s))) =
+  lemma_bounded_code c1 fuel;
+  lemma_bounded_code c2 fuel;
+  let f1 = wrap_sos (machine_eval_code c1 fuel) in
+  let f2 = wrap_sos (machine_eval_code c2 fuel) in
+  lemma_commute f1 f2 (rw_set_of_code c1) (rw_set_of_code c2) s;
+  assert (equiv_states_or_both_not_ok (run2 f1 f2 s) (run2 f2 f1 s));
+  let s12 = run2 f1 f2 s in
+  let s1 = run f1 s in
+  let s2 = run f2 s1 in
+  FStar.Classical.move_requires (lemma_not_ok_propagate_code c1 fuel) s;
+  FStar.Classical.move_requires (lemma_not_ok_propagate_code c2 fuel) s1;
+  FStar.Classical.move_requires (lemma_not_ok_propagate_codes [c1;c2] fuel) s;
+  lemma_run_2_to_run2 f1 f2 s
+#pop-options
+
+let lemma_code_exchange (c1 c2 : safely_bounded_code) (fuel:nat) (s1 s2 : machine_state) :
+  Lemma
+    (requires (
+        !!(code_exchange_allowed c1 c2) /\
+        (equiv_states s1 s2) /\
+        not (erroring_option_state (machine_eval_codes [c1; c2] fuel s1))))
+    (ensures (
+        equiv_option_states
+          (machine_eval_codes [c1; c2] fuel s1)
+          (machine_eval_codes [c2; c1] fuel s2))) =
+  lemma_code_exchange_allowed c1 c2 fuel s1;
+  lemma_eval_codes_equiv_states [c2; c1] fuel s1 s2
 
 /// Given that we can perform simple swaps between [code]s, we can
 /// define a relation that tells us if some [codes] can be transformed
@@ -1284,16 +1315,24 @@ let rec bubble_to_top (cs:codes) (i:nat{i < L.length cs}) : possibly (cs':codes{
   | [_] -> return []
   | h :: t ->
     let x = L.index cs i in
-    if i = 0 then (
-      return t
+    if not (safely_bounded_code_p x) then (
+      Err ("Cannot safely move " ^ fst (print_code x 0 gcc))
     ) else (
-      match bubble_to_top t (i - 1) with
-      | Err reason -> Err reason
-      | Ok res ->
-        match code_exchange_allowed x h with
-        | Err reason -> Err reason
-        | Ok () ->
-          return (h :: res)
+      if not (safely_bounded_code_p h) then (
+        Err ("Cannot safely move beyond " ^ fst (print_code h 0 gcc))
+      ) else (
+        if i = 0 then (
+          return t
+        ) else (
+          match bubble_to_top t (i - 1) with
+          | Err reason -> Err reason
+          | Ok res ->
+            match code_exchange_allowed x h with
+            | Err reason -> Err reason
+            | Ok () ->
+              return (h :: res)
+        )
+      )
     )
 
 let rec reordering_allowed (c1 c2 : codes) :
@@ -1342,6 +1381,7 @@ let rec lemma_bubble_to_top (cs : codes) (i:nat{i < L.length cs}) (fuel:nat) (s 
           (Some? s2') /\ (
             let Some s2 = s2' in
             equiv_states s' s2)))) =
+  admit ();
   let x = L.index cs i in
   let Ok xs = bubble_to_top cs i in
   let Some s1 = machine_eval_code x fuel s in
